@prefix dc: <http://purl.org/dc/elements/1.1/> .
@prefix dcterms: <http://purl.org/dc/terms/> .
@prefix rdf: <http://www.w3.org/1999/02/22-rdf-syntax-ns#> .
@prefix rdfs: <http://www.w3.org/2000/01/rdf-schema#> .
@prefix skos: <http://www.w3.org/2004/02/skos/core#> .
@prefix skosxl: <http://www.w3.org/2008/05/skos-xl#> .
@prefix xml: <http://www.w3.org/XML/1998/namespace> .
@prefix xsd: <http://www.w3.org/2001/XMLSchema#> .
@prefix vann: <http://purl.org/vocab/vann/> .
@prefix vs: <http://www.w3.org/2003/06/sw-vocab-status/ns#> .
@prefix adms: <http://www.w3.org/ns/adms#> .
@prefix lrmi: <http://purl.org/dcx/lrmi-vocabs/learningResourceType/> .
@prefix dcpet: <http://purl.org/dcx/pet/learningResourceType/> .
@prefix bibo: <http://purl.org/ontology/bibo/status/> .

#=============================
# DCPET "LEARNING RESOURCE TYPE" CONCEPT SCHEME DESCRIPTION
#=============================

dcpet: a skos:ConceptScheme ;
    dc:title "DC-PET Learning Resource Type Vocabulary"@en-US ;
    dc:creator "LD4PE Task Group (DCMI)"@en-US ;
    dcterms:dateSubmitted "2015-10-08"^^xsd:date ; 
    dc:description "A concept scheme defining the predominant genre, type or kind characterizing a learning resource"@en-US ;
    dc:source "Extension of LRMI Learning Resource Type Vocabulary at http://purl.org/dcx/lrmi-vocabs/learningResourceType/"@en-US ;
    adms:status bibo:draft .
    
#=============================
# DCPET CONCEPTS
#=============================
    
dcpet:dataset a skos:Concept ;
    skos:prefLabel "dataset"@en-US ;
    skosxl:prefLabel dcpet:label-dataset ; 
    skos:definition "Visual, factual, or numerical information that comes from a sensing device, whether instrument-measured or human-observed; describes both unprocessed, \"raw\" information as well as information already organized into lists, tables, or databases."@en-US ;
    skos:inScheme dcpet: ;
    dcterms:source "Definition based on NSDL (https://wiki.ucar.edu/display/nsdldocs/Type)."@en-US ;
    vs:term_status "unstable" . 
    
dcpet:lecture-presentation a skos:Concept ;
    skos:prefLabel "lecture/presentation"@en-US ;
    skosxl:prefLabel dcpet:label-lecture-presentation ; 
    skos:definition "Audio or text record of a speech or a unit of instruction organized and delivered by an instructor for the purpose of informing a group about a topic."@en-US ;
    skos:inScheme dcpet: ;
    dcterms:source "Definition based on NSDL (https://wiki.ucar.edu/display/nsdldocs/Type)."@en-US ;
    vs:term_status "unstable" .  
    
dcpet:lessonPlan a skos:Concept ;
    skos:prefLabel "lesson plan"@en-US ;
    skosxl:prefLabel dcpet:label-lessonPlan ; 
    skos:definition "Resource to support students' learning of specific concepts, skills, or content; often includes teaching instructions, educational goals, learning objectives, and procedures"@en-US ;
    skos:broader lrmi:lesson ;
    skos:inScheme dcpet: ;
    dcterms:source "Definition based on NSDL (https://wiki.ucar.edu/display/nsdldocs/Type)."@en-US ;
    vs:term_status "unstable" .        
    
dcpet:screencast a skos:Concept ;
    skos:prefLabel "screencast"@en-US ;
    skosxl:prefLabel dcpet:label-screencast ; 
    skos:definition "An event digitally recorded as a set of moving images for later access and presentation."@en-US ;
    vann:usageNote "Use \"screencast\" to describe recorded video of a learning event in the form of a broadcast, lecture, learning activity, tutorial, workshop, or webinar. The recorded event may be with our without an audience present at the time of recording."@en-US ;
    skos:inScheme dcpet: ;
    vs:term_status "unstable" .
    
dcpet:syllabus a skos:Concept ;
    skos:prefLabel "syllabus"@en-US ;
    skosxl:prefLabel dcpet:label-syllabus ; 
    skos:definition "Plan showing the structure of a particular course, including course description and objectives, grading policy, materials, assignments, lesson sequence, and course calendar."@en-US ;
    skos:inScheme dcpet: ;
    skos:broader lrmi:educatorCurriculumGuide ;
    dcterms:source "Definition based on NSDL (https://wiki.ucar.edu/display/nsdldocs/Type)."@en-US ;
    vs:term_status "unstable" .                    
    
#=============================
# CONTEPTS INCLUDED FROM LRMI CONCEPT SCHEME FOR LEARNING RESOURCE TYPE
# @ <http://purl.org/dcx/pet/learningResourceType/>
#=============================

lrmi:alternateAssessment skos:inScheme dcpet: .

lrmi:assessmentItem skos:inScheme dcpet: .
       
lrmi:course skos:inScheme dcpet: .

lrmi:demonstration-simulation skos:inScheme dcpet: .
    
lrmi:educatorCurriculumGuide skos:inScheme dcpet: .
    
lrmi:formativeAssessment skos:inScheme dcpet: .

lrmi:images-visuals skos:inScheme dcpet: .
    
lrmi:interim-summativeAssessment skos:inScheme dcpet: .   

lrmi:learningActivity skos:inScheme dcpet: .   

lrmi:lesson skos:inScheme dcpet: .    

lrmi:primarySource skos:inScheme dcpet: .         

lrmi:rubricScoringGuide skos:inScheme dcpet: .

lrmi:selfAssessment skos:inScheme dcpet: .

lrmi:text skos:inScheme dcpet: .

lrmi:textbook skos:inScheme dcpet: .      
 
lrmi:unit skos:inScheme dcpet: .
    
#============================= 
# EXTENDED LABELS
#=============================    
    
dcpet:label-dataset a skosxl:label ;
    skosxl:literalForm "dataset"@en-US .
    
dcpet:label-lecture-presentation a skosxl:label ;
    skosxl:literalForm "lecture-presentation"@en-US .
    
dcpet:label-lessonPlan a skosxl:label ;
    skosxl:literalForm "lesson plan"@en-US .    
    
dcpet:label-screencast a skosxl:label ;
    skosxl:literalForm "screencast"@en-US .
    
dcpet:label-syllabus a skosxl:label ;
    skosxl:literalForm "syllabus"@en-US .                 
        
 
